redesign low-level code

code/mpfr/MPFR.Add.Spec.fst
@@ -1,106 +1,57 @@
 module MPFR.Add.Spec
 
 open FStar.Mul
+open MPFR.BinaryFP
 open MPFR.Lib.Spec
+open MPFR.Maths
 
 #set-options "--z3refresh --z3rlimit 5 --max_fuel 1 --initial_fuel 0 --max_ifuel 1 --initial_ifuel 0"
 
-(* Proprieties for addition *)
-val add: a:floating_point ->
-         b:floating_point{a.sign = b.sign} ->
-    Tot (r:floating_point{r.sign = a.sign /\
-          (let elb = min a.exp b.exp in
-	   r.exp >= elb /\
-           (a.mant * pow2 (a.exp - elb)) +
-	   (b.mant * pow2 (b.exp - elb)) =
-	   (r.mant * pow2 (r.exp - elb)))})
-
-(* Implementation for addition *)
-private let min (a:int) (b:int) = if a >= b then b else a
-private let max (a:int) (b:int) = if a >= b then a else b
-
-val add_mant: a:floating_point ->
-              b:floating_point{a.sign = b.sign} ->
-	  Tot nat
-let add_mant a b =
-    if a.exp >= b.exp then a.mant * pow2 (a.exp - b.exp) + b.mant
-                     else b.mant * pow2 (b.exp - a.exp) + a.mant
+(* Useful functions when adding two MPFR numbers with same precision
+ * and the exponent of the first one is greater than that of the second one *)
+val add_sp_ge_limb: a:mpfr_fp -> b:mpfr_fp -> Pure nat
+    (requires (a.sign = b.sign /\ a.prec = b.prec /\ a.exp >= b.exp))
+    (ensures  (fun rm -> rm = abs (eval a +. eval b).significand /\
+                      rm % pow2 (a.len - a.prec) = 0))
     
-val add_exp : a:floating_point ->
-              b:floating_point{a.sign = b.sign} ->
-	 Tot (r:int{r >= min a.exp b.exp})
-let add_exp a b = min a.exp b.exp
+let add_sp_ge_limb a b =
+    lemma_mul_mod a.limb (pow2 (a.exp - b.exp)) (pow2 (a.len - a.prec));
+    lemma_mod_distr (a.limb * pow2 (a.exp - b.exp)) b.limb (pow2 (a.len - a.prec));
+    a.limb * pow2 (a.exp - b.exp) + b.limb
+    
+val add_sp_ge_exp: a:mpfr_fp -> b:mpfr_fp -> Pure int
+    (requires (a.sign = b.sign /\ a.prec = b.prec /\ a.exp >= b.exp))
+    (ensures  (fun rx -> rx - bits (add_sp_ge_limb a b) = (eval a +. eval b).exponent))
 
-val add_prec: a:floating_point ->
-              b:floating_point{a.sign = b.sign} ->
-	  Tot (p:nat{let p0 = if a.exp >= b.exp then max (a.prec + a.exp - b.exp) b.prec 
-                                             else max (b.prec + b.exp - a.exp) a.prec in
-	           p0 <= p /\ p <= p0 + 1})
-let add_prec a b =
-    let p0 = if a.exp >= b.exp then max (a.prec + a.exp - b.exp) b.prec 
-                              else max (b.prec + b.exp - a.exp) a.prec in
-    if add_mant a b < pow2 p0 then p0 else p0 + 1
-
-
-open MPFR.Lemmas
-
-(* Useful lemmas *)
-val add_fp_lemma: a:floating_point ->
-                  b:floating_point{a.sign = b.sign} ->
-    Lemma (let sp = add_prec a b in
-           let sm = add_mant a b in
-	   pow2 (sp - 1) <= sm /\ sm < pow2 sp)
-let add_fp_lemma a b =
-    let sp = add_prec a b in
-    let sm = add_mant a b in
-    let p0 = if a.exp >= b.exp then max (a.prec + a.exp - b.exp) b.prec 
-                              else max (b.prec + b.exp - a.exp) a.prec in
-    if sm < pow2 p0 then begin
-	if a.exp >= b.exp then begin
-	    lemma_mul_le_right (pow2 (a.exp - b.exp)) (pow2 (a.prec - 1)) a.mant;
-	    lemma_pow2_mul (a.prec - 1) (a.exp - b.exp)
-	end else begin
-	    lemma_mul_le_right (pow2 (b.exp - a.exp)) (pow2 (b.prec - 1)) b.mant;
-	    lemma_pow2_mul (b.prec - 1) (b.exp - a.exp)
-	end
+let add_sp_ge_exp a b =
+    let d = a.exp - b.exp in
+    if add_sp_ge_limb a b < pow2 (bits a.limb + d) then begin 
+	lemma_mul_le_right (pow2 d) (pow2 (bits a.limb - 1)) a.limb;
+	lemma_pow2_mul (bits a.limb - 1) d;
+	lemma_log2_le (pow2 (bits a.limb - 1 + d)) (add_sp_ge_limb a b);
+	lemma_log2_lt (add_sp_ge_limb a b) (bits a.limb + d);
+        a.exp
     end else begin
-	if a.exp >= b.exp then begin
-	    lemma_mul_lt_right (pow2 (a.exp - b.exp)) a.mant (pow2 a.prec);
-	    lemma_pow2_mul a.prec (a.exp - b.exp);
-	    lemma_pow2_le (a.prec + a.exp - b.exp) (max (a.prec + a.exp - b.exp) b.prec);
-	    lemma_pow2_le b.prec (max (a.prec + a.exp - b.exp) b.prec);
-	    lemma_pow2_double (max (a.prec + a.exp - b.exp) b.prec)
-	end else begin
-	    lemma_mul_lt_right (pow2 (b.exp - a.exp)) b.mant (pow2 b.prec);
-	    lemma_pow2_mul b.prec (b.exp - a.exp);
-	    lemma_pow2_le (b.prec + b.exp - a.exp) (max (b.prec + b.exp - a.exp) a.prec);
-	    lemma_pow2_le a.prec (max (b.prec + b.exp - a.exp) a.prec);
-	    lemma_pow2_double (max (b.prec + b.exp - a.exp) a.prec)
-	end
+	lemma_log2_le (pow2 (bits a.limb + d)) (add_sp_ge_limb a b);
+        lemma_mul_lt_right (pow2 d) a.limb (pow2 (bits a.limb));
+        lemma_pow2_mul (bits a.limb) d;
+	lemma_pow2_le (bits b.limb) (bits a.limb + d);
+        lemma_pow2_double (bits a.limb + d);
+	lemma_log2_lt (add_sp_ge_limb a b) (bits a.limb + d + 1);
+        a.exp + 1
     end
+    
+val add_sp_ge_prec: a:mpfr_fp -> b:mpfr_fp -> Pure pos
+    (requires (a.sign = b.sign /\ a.prec = b.prec /\ a.exp >= b.exp))
+    (ensures  (fun rp -> bits (add_sp_ge_limb a b) - rp = bits a.limb - a.prec))
+    
+let add_sp_ge_prec a b = a.prec + add_sp_ge_exp a b - b.exp
 
-val add_value_lemma: a:floating_point ->
-                     b:floating_point{a.sign = b.sign} ->
-    Lemma (let elb = min a.exp b.exp in
-           add_exp a b >= elb /\
-           (a.mant * pow2 (a.exp - elb)) +
-	   (b.mant * pow2 (b.exp - elb)) =
-	   (add_mant a b * pow2 (add_exp a b - elb)))
-let add_value_lemma a b = 
-    let sx = add_exp a b in
-    let sm = add_mant a b in
-    let elb = min a.exp b.exp in
-    if a.exp >= b.exp then begin
-        lemma_distr_add_left (a.mant * pow2 (a.exp - b.exp)) b.mant (pow2 (sx - elb));
-	lemma_paren_mul_right a.mant (pow2 (a.exp - b.exp)) (pow2 (sx - elb));
-	lemma_pow2_mul (a.exp - b.exp) (sx - elb)
-    end else begin
-        lemma_distr_add_left (b.mant * pow2 (b.exp - a.exp)) a.mant (pow2 (sx - elb));
-	lemma_paren_mul_right b.mant (pow2 (b.exp - a.exp)) (pow2 (sx - elb));
-	lemma_pow2_mul (b.exp - a.exp) (sx - elb)
-    end
-
-let add a b = 
-    add_fp_lemma a b;
-    add_value_lemma a b;
-    {sign = a.sign; prec = add_prec a b; mant = add_mant a b; exp = add_exp a b}
+(* Addition for two MPFR numbers with same precision *)
+val add_sp: a:mpfr_fp -> b:mpfr_fp -> Pure ieee_fp
+    (requires (a.sign = b.sign /\ a.prec = b.prec))
+    (ensures  (fun r -> eval a +. eval b =. eval r))
+    
+let add_sp a b = 
+    let a, b = if a.exp >= b.exp then a, b else b, a in
+    mk_ieee a.sign (add_sp_ge_prec a b) (add_sp_ge_exp a b) (add_sp_ge_limb a b) (bits (add_sp_ge_limb a b))
