code/mpfr/MPFR.Lib.Spec.fst
@@ -1,26 +1,94 @@
 module MPFR.Lib.Spec
 
 open FStar.Mul
+open MPFR.BinaryFP
+open MPFR.Maths
 
-(* This struct describe a number: sign * mant * 2^exp *)
+#set-options "--z3refresh --z3rlimit 5 --max_fuel 1 --initial_fuel 0 --max_ifuel 1 --initial_ifuel 0"
+
+
+///////////////////////////////////////////////////////
+//  Struct Definition                                //
+//  Used to store IEEE format floating point number  //
+///////////////////////////////////////////////////////
+
+(* Note that 0 is not supported *)
 type fp_struct = {
-    sign: s:int{s = 1 \/ s = -1};
+    sign: (s:int{s = -1 \/ s = 1});
     prec: pos;
-    mant: nat;
-    exp : int
+    exp : int;
+    limb: nat;
+    len : pos;
 }
 
-(* Condition for validity *)
-let fp_cond (s:fp_struct) = pow2 (s.prec - 1) <= s.mant /\ s.mant < pow2 s.prec
-type floating_point = s:fp_struct{fp_cond s}
+let mk_struct sign prec exp limb len = {
+    sign = sign;
+    prec = prec;
+    exp  = exp;
+    limb = limb;
+    len  = len
+}
+
+(* Get bit length of a positive integer *)
+val bits: m:pos -> Tot (p:pos{pow2 (p - 1) <= m /\ m < pow2 p})
+let bits m = log2 m + 1
+
+type valid_struct = s:fp_struct{s.limb = 0 \/ bits s.limb <= s.len}
+
+(* Evaluation. Here is the method.
+ * Firstly add '0.' in front of 'limb' to make it a floating number in (0, 1)
+ * Then multiply it with 2 ^ exp *)
+let eval (fp:fp_struct) = mk_fp (fp.sign * fp.limb) (fp.exp - fp.len)
+
+
+/////////////////////////////////////////////////////////////////////////////////////////
+//  Validity Test for ieee_struct                                                      //
+//  A valid struct represents a binary floating point number defined in MPFR.BinaryFP  //
+//  Important function 'eval' maps ieee_fp to binary_fp                                //
+/////////////////////////////////////////////////////////////////////////////////////////
+
+(* Condition for validity 
+ * A valid struct should have a positive precision which is smaller than 'limb' length
+ * Only the first 'prec' bits of 'limb' store value and the rest bits are 0s *)
+let ieee_valid_cond (s:fp_struct) =
+    s.limb > 0 /\ bits s.limb = s.len /\
+    0 < s.prec /\ s.prec <= s.len /\
+    s.limb % pow2 (s.len - s.prec) = 0
+    
+type ieee_fp = s:valid_struct{ieee_valid_cond s}
+
+let mk_ieee sign prec exp limb len: Pure ieee_fp
+    (requires (ieee_valid_cond (mk_struct sign prec exp limb len)))
+    (ensures  (fun _ -> True)) =
+    mk_struct sign prec exp limb len
+
+
+//////////////////////////////////////////////////////
+//  A special type corresponding to top level code  //
+//  Pure version of mpfr_struct                     //
+//////////////////////////////////////////////////////
 
 (* Condition for parameters range corresponding to top level code *)
-let mpfr_PREC_MIN_P = 1
-let mpfr_PREC_MAX_P = 63
-let mpfr_EMIN_P = 1 - pow2 30 - mpfr_PREC_MAX_P
-let mpfr_EMAX_P = pow2 30 - 1 - mpfr_PREC_MIN_P
-let mpfr_range_cond (s:floating_point) =
-    mpfr_PREC_MIN_P <= s.prec /\ s.prec <= mpfr_PREC_MAX_P /\
-    mpfr_EMIN_P <= s.exp /\ s.exp <= mpfr_EMAX_P
+let gmp_NUMB_BITS = 64
+let mpfr_PREC_MIN = 1
+let mpfr_PREC_MAX = pow2 31 - 1
+let mpfr_PREC_COND (p:pos) = mpfr_PREC_MIN <= p /\ p <= mpfr_PREC_MAX
 
-type mpfr_fp = f:floating_point{mpfr_range_cond f}
+let mpfr_EXP_INVALID = pow2 30
+let mpfr_EMIN = 1 - mpfr_EXP_INVALID
+let mpfr_EMAX = mpfr_EXP_INVALID - 1
+let mpfr_EXP_COND (x:int) = mpfr_EMIN <= x /\ x <= mpfr_EMAX
+
+(* Condition for a MPFR floating number
+ * The precision and exponent have range limits
+ * The bit length of limb must be a multiple of 64 and as small as possible *)
+val arr_size: p:pos ->
+    Tot (s:pos{s % 64 = 0 /\ s >= p /\ s - 64 < p})
+let arr_size p = ((p + 63) / 64) * 64
+
+let mpfr_valid_cond (s:ieee_fp) =
+    s.len = arr_size s.prec /\
+    mpfr_PREC_COND s.prec /\
+    mpfr_EXP_COND s.exp
+
+type mpfr_fp = f:ieee_fp{mpfr_valid_cond f}
