code/mpfr/MPFR.Maths.fst
@@ -1,4 +1,4 @@
-module MPFR.Lemmas
+module MPFR.Maths
 
 open FStar.Mul
 
@@ -9,173 +9,105 @@ open FStar.Mul
 (* Nonlinear arithmetic *)
 val lemma_paren_mul_left: a:int -> b:int -> c:int -> Lemma
     (a * b * c = (a * b) * c)
+let lemma_paren_mul_left a b c = ()
 
 val lemma_paren_mul_right: a:int -> b:int -> c:int -> Lemma
     (a * b * c = a * (b * c))
+let lemma_paren_mul_right a b c = ()
 
 val lemma_mul_le_left: a:nat -> b:int -> c:int -> Lemma
     (requires (b <= c))
     (ensures  (a * b <= a * c))
+let lemma_mul_le_left a b c = ()
 
 val lemma_mul_le_right: a:nat -> b:int -> c:int -> Lemma
     (requires (b <= c))
     (ensures  (b * a <= c * a))
+let lemma_mul_le_right a b c = ()
 
 val lemma_mul_lt_left: a:pos -> b:int -> c:int -> Lemma
     (requires (b < c))
     (ensures  (a * b < a * c))
+let lemma_mul_lt_left a b c = ()
 
 val lemma_mul_lt_right: a:pos -> b:int -> c:int -> Lemma
     (requires (b < c))
     (ensures  (b * a < c * a))
+let lemma_mul_lt_right a b c = ()
 
 val lemma_distr_add_left: a:int -> b:int -> c:int -> Lemma
     ((a + b) * c = a * c + b * c)
+let lemma_distr_add_left a b c = ()
 
 val lemma_distr_add_right: a:int -> b:int -> c:int -> Lemma
     (a * (b + c) = a * b + a * c)
+let lemma_distr_add_right a b c = ()
 
 val lemma_distr_sub_left: a:int -> b:int -> c:int -> Lemma
     ((a - b) * c = a * c - b * c)
+let lemma_distr_sub_left a b c = ()
 
 val lemma_distr_sub_right: a:int -> b:int -> c:int -> Lemma
     (a * (b - c) = a * b - a * c)
-
-(* Division and modulo *)
-val lemma_small_div: a:nat -> b:pos -> Lemma
-    (requires (a < b))
-    (ensures  (a / b = 0))
-
-val lemma_small_mod: a:nat -> b:pos -> Lemma
-    (requires (a < b))
-    (ensures  (a % b = a))
-
-val lemma_multiple_div: a:nat -> b:pos -> Lemma
-    ((a * b) / b = a)
-
-val lemma_multiple_mod: a:nat -> b:pos -> Lemma
-    ((a * b) % b = 0)
-
-val lemma_div_lt: a:nat -> b:nat -> d:pos -> Lemma
-    (requires (a < b /\ b % d = 0))
-    (ensures  (a / d < b / d))
-
-val lemma_div_le: a:nat -> b:nat -> d:pos -> Lemma
-    (requires (a <= b))
-    (ensures  (a / d <= b / d))
-
-val lemma_div_distr: a:nat -> b:nat -> c:pos -> Lemma
-    (requires (a % c = 0))
-    (ensures  ((a + b) / c = a / c + b / c))
-
-val lemma_mod_distr: a:nat -> b:nat -> c:pos -> Lemma
-    ((a + b) % c = (a % c + b % c) % c)
-
-val lemma_div_div: a:nat -> b:pos -> c:pos -> Lemma
-    ((a / b) / c = a / (b * c))
-
-val lemma_mul_div: a:nat -> b:nat -> c:pos -> Lemma
-    (requires (a % c = 0))
-    (ensures  ((a * b) / c = (a / c) * b))
-    
-val lemma_mod_div: a:nat -> b:pos -> c:pos -> Lemma 
-    ((a % (b * c)) / b = (a / b) % c)
-
-val lemma_mod_mod: a:nat -> b:pos -> c:pos -> Lemma
-    ((a % (b * c)) % b = a % b)
-
-(* pow2 proprieties *)
-val lemma_pow2_le: n:nat -> m:nat -> Lemma
-    (requires (n <= m))
-    (ensures  (pow2 n <= pow2 m))
-
-val lemma_pow2_lt: n:nat -> m:nat -> Lemma
-    (requires (n < m))
-    (ensures  (pow2 n < pow2 m))
-    
-val lemma_pow2_le_inv: n:nat -> m:nat -> Lemma
-    (pow2 n <= pow2 m ==> n <= m)
-
-val lemma_pow2_lt_inv: n:nat -> m:nat -> Lemma
-    (pow2 n < pow2 m ==> n < m)
-    
-val lemma_pow2_mul: n:nat -> m:nat -> Lemma
-    (pow2 n * pow2 m = pow2 (n + m))
-
-val lemma_pow2_small_div: n:nat -> m:nat -> Lemma
-    (requires (n < m))
-    (ensures  (pow2 n / pow2 m = 0))
-
-val lemma_pow2_small_mod: n:nat -> m:nat -> Lemma
-    (requires (n < m))
-    (ensures  (pow2 n % pow2 m = pow2 n))
-
-val lemma_pow2_div: n:nat -> m:nat -> Lemma
-    (requires (m <= n))
-    (ensures  (pow2 n / pow2 m = pow2 (n - m)))
-
-val lemma_pow2_mod: n:nat -> m:nat -> Lemma
-    (requires (m <= n))
-    (ensures  (pow2 n % pow2 m = 0))
-
-val lemma_pow2_double: n:nat -> Lemma
-    (pow2 n + pow2 n = pow2 (n + 1))
-
-val lemma_pow2_div_lt: a:nat -> b:nat -> d:nat -> Lemma
-    (requires (a < pow2 b /\ d <= b))
-    (ensures  (a / pow2 d < pow2 (b - d)))
-
-val lemma_pow2_div_div: a:nat -> b:nat -> c:nat -> Lemma
-    ((a / pow2 b) / pow2 c = a / pow2 (b + c))
-
-val lemma_pow2_mod_div: a:nat -> b:nat -> c:nat -> Lemma
-    (requires (b >= c))
-    (ensures  ((a % pow2 b) / pow2 c = (a / pow2 c) % (pow2 (b - c))))
-
-val lemma_pow2_mod_mod: a:nat -> b:nat -> c:nat -> Lemma
-    (requires (b >= c))
-    (ensures  ((a % pow2 b) % pow2 c = a % pow2 c))
-    
-
-(* Proofs *)
-(* Nonlinear arithmetic *)
-let lemma_paren_mul_left a b c = ()
-let lemma_paren_mul_right a b c = ()
-let lemma_mul_le_left a b c = ()
-let lemma_mul_le_right a b c = ()
-let lemma_mul_lt_left a b c = ()
-let lemma_mul_lt_right a b c = ()
-let lemma_distr_add_left a b c = ()
-let lemma_distr_add_right a b c = ()
-let lemma_distr_sub_left a b c = ()
 let lemma_distr_sub_right a b c = ()
 
 (* Division and modulo *)
 val lemma_euclidean: a:nat -> b:pos -> Lemma
     (a = (a / b) * b + a % b)
 let lemma_euclidean a b = ()
+
 val lemma_add_div: a:nat -> n:int -> d:pos -> Lemma
     (requires (a + n * d >= 0))
     (ensures  ((a + n * d) / d = a / d + n))
 let lemma_add_div a n d = assert(a / d + n - 1 < (a + n * d) / d /\ (a + n * d) / d < a / d + n + 1)
+
 val lemma_add_mod: a:nat -> n:int -> d:pos -> Lemma
     (requires (a + n * d >= 0))
     (ensures  ((a + n * d) % d = a % d))
 let lemma_add_mod a n d = lemma_add_div a n d
 
+val lemma_small_div: a:nat -> b:pos -> Lemma
+    (requires (a < b))
+    (ensures  (a / b = 0))
 let lemma_small_div a b = ()
+
+val lemma_small_mod: a:nat -> b:pos -> Lemma
+    (requires (a < b))
+    (ensures  (a % b = a))
 let lemma_small_mod a b = ()
+
+val lemma_multiple_div: a:nat -> b:pos -> Lemma
+    ((a * b) / b = a)
 let lemma_multiple_div a b = lemma_add_div 0 a b
+
+val lemma_multiple_mod: a:nat -> b:pos -> Lemma
+    ((a * b) % b = 0)
 let lemma_multiple_mod a b = lemma_multiple_div a b
+
+val lemma_div_lt: a:nat -> b:nat -> d:pos -> Lemma
+    (requires (a < b /\ b % d = 0))
+    (ensures  (a / d < b / d))
 let lemma_div_lt a b d = assert(a / d >= b / d ==> a >= b)
+
+val lemma_div_le: a:nat -> b:nat -> d:pos -> Lemma
+    (requires (a <= b))
+    (ensures  (a / d <= b / d))
 let lemma_div_le a b d = lemma_add_div (b - a / d * d) (a / d) d
+
+val lemma_div_distr: a:nat -> b:nat -> c:pos -> Lemma
+    (requires (a % c = 0))
+    (ensures  ((a + b) / c = a / c + b / c))
 let lemma_div_distr a b c = lemma_add_div b (a / c) c
 
+val lemma_mod_distr: a:nat -> b:nat -> c:pos -> Lemma
+    ((a + b) % c = (a % c + b % c) % c)
 let lemma_mod_distr a b c =
     lemma_euclidean a c;
     //! assert((a + b) / c = ((a / c + b / c) * c + (a % c + b % c)) / c);
     lemma_add_mod (a % c + b % c) (a / c + b / c) c
-    
+
+val lemma_div_div: a:nat -> b:pos -> c:pos -> Lemma
+    ((a / b) / c = a / (b * c))
 let lemma_div_div a b c =
     lemma_euclidean a b;
     //! assert(a = (a / b) * b + a % b);
@@ -188,11 +120,21 @@ let lemma_div_div a b c =
     //! assert(((a / b) % c) * b + a % b <= (c - 1) * b + (b - 1));
     lemma_small_div (((a / b) % c) * b + a % b) (b * c)
 
+val lemma_mul_div: a:nat -> b:nat -> c:pos -> Lemma
+    (requires (a % c = 0))
+    (ensures  ((a * b) / c = (a / c) * b))
 let lemma_mul_div a b c =
     lemma_euclidean a c;
     //! assert((a * b) / c = ((a / c) * c * b) / c);
     lemma_multiple_div ((a / c) * b) c
 
+val lemma_mul_mod: a:nat -> b:nat -> c:pos -> Lemma
+    (requires (a % c = 0))
+    (ensures  ((a * b) % c = 0))
+let lemma_mul_mod a b c = lemma_mul_div a b c
+    
+val lemma_mod_div: a:nat -> b:pos -> c:pos -> Lemma 
+    ((a % (b * c)) / b = (a / b) % c)
 let lemma_mod_div a b c =
     lemma_euclidean a (b * c);
     //! assert(a = (a / (b * c)) * (b * c) + a % (b * c));
@@ -202,41 +144,131 @@ let lemma_mod_div a b c =
     //! assert((a % (b * c)) / b = a / b - ((a / b) / c) * c);
     lemma_euclidean (a / b) c
 
+val lemma_mod_mod: a:nat -> b:pos -> c:pos -> Lemma
+    ((a % (b * c)) % b = a % b)
 let lemma_mod_mod a b c =
     lemma_euclidean a (b * c);
     lemma_add_mod a (- (a / (b * c)) * c) b
 
 (* pow2 proprieties *)
+val lemma_pow2_le: n:nat -> m:nat -> Lemma
+    (requires (n <= m))
+    (ensures  (pow2 n <= pow2 m))
 let lemma_pow2_le n m = FStar.Math.Lemmas.pow2_le_compat m n
+
+val lemma_pow2_lt: n:nat -> m:nat -> Lemma
+    (requires (n < m))
+    (ensures  (pow2 n < pow2 m))
 let lemma_pow2_lt n m = FStar.Math.Lemmas.pow2_lt_compat m n
-let lemma_pow2_le_inv n m = if m < n then lemma_pow2_lt m n else ()
-let lemma_pow2_lt_inv n m = if m <= n then lemma_pow2_le m n else ()
+    
+val lemma_pow2_mul: n:nat -> m:nat -> Lemma
+    (pow2 n * pow2 m = pow2 (n + m))
 let lemma_pow2_mul n m = FStar.Math.Lemmas.pow2_plus n m
+
+val lemma_pow2_small_div: n:nat -> m:nat -> Lemma
+    (requires (n < m))
+    (ensures  (pow2 n / pow2 m = 0))
 let lemma_pow2_small_div n m =
     lemma_pow2_lt n m;
     lemma_small_div (pow2 n) (pow2 m)
+
+val lemma_pow2_small_mod: n:nat -> m:nat -> Lemma
+    (requires (n < m))
+    (ensures  (pow2 n % pow2 m = pow2 n))
 let lemma_pow2_small_mod n m =
     lemma_pow2_lt n m;
     lemma_small_mod  (pow2 n) (pow2 m)
+
+val lemma_pow2_div: n:nat -> m:nat -> Lemma
+    (requires (m <= n))
+    (ensures  (pow2 n / pow2 m = pow2 (n - m)))
 let lemma_pow2_div n m = FStar.Math.Lemmas.pow2_minus n m
+
+val lemma_pow2_mod: n:nat -> m:nat -> Lemma
+    (requires (m <= n))
+    (ensures  (pow2 n % pow2 m = 0))
 let lemma_pow2_mod n m = 
     lemma_pow2_mul (n - m) m;
     lemma_multiple_mod (pow2 (n - m)) (pow2 m)
+
+val lemma_pow2_double: n:nat -> Lemma
+    (pow2 n + pow2 n = pow2 (n + 1))
 let lemma_pow2_double n = ()
+
+val lemma_pow2_div_lt: a:nat -> b:nat -> d:nat -> Lemma
+    (requires (a < pow2 b /\ d <= b))
+    (ensures  (a / pow2 d < pow2 (b - d)))
 let lemma_pow2_div_lt a b d = 
     lemma_pow2_div b d;
     lemma_pow2_mod b d;
     lemma_div_lt a (pow2 b) (pow2 d)
+
+val lemma_pow2_div_div: a:nat -> b:nat -> c:nat -> Lemma
+    ((a / pow2 b) / pow2 c = a / pow2 (b + c))
 let lemma_pow2_div_div a b c =
     lemma_pow2_mul b c;
     lemma_div_div a (pow2 b) (pow2 c)
+
+val lemma_pow2_mod_div: a:nat -> b:nat -> c:nat -> Lemma
+    (requires (b >= c))
+    (ensures  ((a % pow2 b) / pow2 c = (a / pow2 c) % (pow2 (b - c))))
 let lemma_pow2_mod_div a b c =
     lemma_pow2_mul c (b - c);
     lemma_mod_div a (pow2 c) (pow2 (b - c))
+
+val lemma_pow2_mod_mod: a:nat -> b:nat -> c:nat -> Lemma
+    (requires (b >= c))
+    (ensures  ((a % pow2 b) % pow2 c = a % pow2 c))
 let lemma_pow2_mod_mod a b c =
     lemma_pow2_mul c (b - c);
     lemma_mod_mod a (pow2 c) (pow2 (b - c))
 
+(* Function log2 *)
+val log2: a:pos -> n:nat{pow2 n <= a /\ a < pow2 (n + 1)}
+let rec log2 a = if a = 1 then 0 else log2 (a / 2) + 1
+
+val lemma_log2_pow2: n:nat -> Lemma 
+    (ensures (log2 (pow2 n) = n))
+    [SMTPat (log2 (pow2 n))]
+let rec lemma_log2_pow2 n = if n = 0 then () else lemma_log2_pow2 (n - 1)
+
+val lemma_log2_le: a:pos -> b:pos -> Lemma
+    (requires (a <= b))
+    (ensures  (log2 a <= log2 b))
+let rec lemma_log2_le a b = if a = 1 then () else lemma_log2_le (a / 2) (b / 2)
+
+val lemma_log2_lt: a:pos -> b:nat -> Lemma
+    (requires (a < pow2 b))
+    (ensures  (log2 a < b))
+let rec lemma_log2_lt a b = if a < 2 then () else lemma_log2_lt (a / 2) (b - 1)
+
+val lemma_log2_lt_inv: a:pos -> b:pos -> Lemma
+    (requires (log2 a < log2 b))
+    (ensures  (a < b))
+    [SMTPat (log2 a < log2 b)]
+let lemma_log2_lt_inv a b = if a < b then () else lemma_log2_le b a
+
+val lemma_log2_mul: a:pos -> b:nat -> Lemma
+    (ensures (log2 (a * pow2 b) = log2 a + b))
+    [SMTPat (log2 (a * pow2 b))]
+let rec lemma_log2_mul a b = 
+    if b = 0 then () else begin
+        lemma_pow2_div b 1;
+	lemma_mul_div (pow2 b) a 2;
+        lemma_log2_mul a (b - 1)
+    end
+
+val lemma_log2_div: a:pos -> b:nat -> Lemma
+    (requires (log2 a >= b))
+    (ensures  (a / pow2 b > 0 /\ log2 (a / pow2 b) = log2 a - b))
+    [SMTPat (log2 (a / pow2 b))]
+let rec lemma_log2_div a b =
+    if b = 0 then () else begin
+        lemma_pow2_div b 1;
+	lemma_pow2_div_div a (b - 1) 1;
+        lemma_log2_div a (b - 1)
+    end
+    
 
 (* Lemmas about bitwise operations *)
 open FStar.BitVector
